thys/Flyspeck-Tame/ArchCompProps.thy
@@ -64,7 +64,7 @@ proof -
       split:option.splits
       dest: in_set_lookup_of_listD in_set_lookup_set_ofD)
   have "Tries.set_of gs \<subseteq>\<^isub>\<simeq> set arch"
-  proof (auto simp:eqi_gr.defs)
+  proof (auto simp:qle_gr.defs)
     fix g assume g: "g \<in> Tries.set_of gs"
     obtain h where h: "h \<in> set arch" and test: "iso_test g h"
       using test1[OF g] by blast
@@ -73,14 +73,14 @@ proof -
   qed
   moreover
   have "set arch \<subseteq>\<^isub>\<simeq> Tries.set_of gs"
-  proof (auto simp:eqi_gr.defs)
+  proof (auto simp:qle_gr.defs)
     fix g assume g: "g \<in> set arch"
     obtain h where h: "h \<in> Tries.set_of gs" and test: "iso_test g h"
       using test2[OF g] by blast
     thus "\<exists>h \<in> Tries.set_of gs. g \<simeq> h"
       using h pre1[OF _ h] pre2[OF g] by (auto simp:iso_test_correct)
   qed
-  ultimately show ?thesis by (auto simp: eqi_gr.seteq_eqi_def)
+  ultimately show ?thesis by (auto simp: qle_gr.seteq_qle_def)
 qed
 
 lemma samet_imp_iso_subseteq:
@@ -89,30 +89,30 @@ and pre2: "\<And>g. g \<in> set arch \<Longrightarrow> pre_iso_test g"
 and inv: "!!gs. gsopt = Some gs \<Longrightarrow> Tries.inv gs"
 and same: "samet gsopt arch"
 shows "\<exists>gs. gsopt = Some gs \<and> Tries.set_of gs \<subseteq>\<^isub>\<simeq> set arch"
-using eqi_gr.seteq_eqi_def assms samet_imp_iso_seteq by metis
+using qle_gr.seteq_qle_def assms samet_imp_iso_seteq by metis
 
 definition [code del]:
 "insert_mod_trie = set_mod_maps.insert_mod Tries.update Tries.lookup iso_test hash"
 definition [code del]:
-"worklist_dfs_coll_trie = set_modulo.worklist_dfs_coll (Tries [] []) insert_mod_trie"
+"worklist_tree_coll_trie = set_modulo.worklist_tree_coll (Tries [] []) insert_mod_trie"
 definition [code del]:
-"worklist_dfs_coll_aux_trie = set_modulo.worklist_dfs_coll_aux insert_mod_trie"
+"worklist_tree_coll_aux_trie = set_modulo.worklist_tree_coll_aux insert_mod_trie"
 definition [code del]:
 "insert_mod2_trie = set_modulo.insert_mod2 insert_mod_trie"
 
 interpretation set_mod_trie:
   set_mod_maps "Tries [] []" Tries.update Tries.lookup Tries.inv "op \<simeq>" iso_test pre_iso_test hash
-where "set_modulo.worklist_dfs_coll (Tries [] []) insert_mod_trie = worklist_dfs_coll_trie"
-and "set_modulo.worklist_dfs_coll_aux insert_mod_trie = worklist_dfs_coll_aux_trie"
+where "set_modulo.worklist_tree_coll (Tries [] []) insert_mod_trie = worklist_tree_coll_trie"
+and "set_modulo.worklist_tree_coll_aux insert_mod_trie = worklist_tree_coll_aux_trie"
 and "set_mod_maps.insert_mod Tries.update Tries.lookup iso_test hash = insert_mod_trie"
 and "set_modulo.insert_mod2 insert_mod_trie = insert_mod2_trie"
 proof unfold_locales
-qed (auto simp:iso_test_correct worklist_dfs_coll_trie_def worklist_dfs_coll_aux_trie_def insert_mod_trie_def insert_mod2_trie_def)
+qed (auto simp:iso_test_correct worklist_tree_coll_trie_def worklist_tree_coll_aux_trie_def insert_mod_trie_def insert_mod2_trie_def)
 
 definition enum_filter_finals ::
   "(graph \<Rightarrow> graph list) \<Rightarrow> graph list
    \<Rightarrow> (nat,nat fgraph) tries option" where
-"enum_filter_finals succs = set_mod_trie.worklist_dfs_coll succs final fgraph"
+"enum_filter_finals succs = set_mod_trie.worklist_tree_coll succs final fgraph"
 
 definition tameEnumFilter :: "nat \<Rightarrow> (nat,nat fgraph)tries option" where
 "tameEnumFilter p = enum_filter_finals (next_tame p) [Seed p]"
@@ -120,7 +120,7 @@ definition tameEnumFilter :: "nat \<Rightarrow> (nat,nat fgraph)tries option" wh
 lemma TameEnum_tameEnumFilter:
   "tameEnumFilter p = Some t \<Longrightarrow>  Tries.set_of t  =\<^isub>\<simeq> fgraph ` TameEnum\<^bsub>p\<^esub>"
 apply(auto simp: tameEnumFilter_def TameEnumP_def enum_filter_finals_def)
-apply(drule set_mod_trie.worklist_dfs_coll_equiv[OF _ inv_inv_next_tame])
+apply(drule set_mod_trie.worklist_tree_coll_equiv[OF _ inv_inv_next_tame])
 apply (auto simp: Tries.set_of_conv inv_Seed mgp_pre_iso_test RTranCl_conv)
 done
 
@@ -128,19 +128,19 @@ lemma tameEnumFilter_subseteq_TameEnum:
   "tameEnumFilter p = Some t \<Longrightarrow> Tries.set_of t <= fgraph ` TameEnum\<^bsub>p\<^esub>"
 by(auto simp add:tameEnumFilter_def TameEnumP_def enum_filter_finals_def
      Tries.set_of_conv inv_Seed mgp_pre_iso_test RTranCl_conv
-     dest!: set_mod_trie.worklist_dfs_coll_subseteq[OF _ inv_inv_next_tame])
+     dest!: set_mod_trie.worklist_tree_coll_subseteq[OF _ inv_inv_next_tame])
 
 
 lemma inv_tries_tameEnumFilter:
   "tameEnumFilter p = Some t \<Longrightarrow> Tries.inv t"
 unfolding tameEnumFilter_def enum_filter_finals_def
-by(erule set_mod_trie.worklist_dfs_coll_inv)
+by(erule set_mod_trie.worklist_tree_coll_inv)
 
 theorem combine_evals_filter:
  "\<forall>g \<in> set arch. pre_iso_test g \<Longrightarrow> samet (tameEnumFilter p) arch
   \<Longrightarrow> fgraph ` TameEnum\<^bsub>p\<^esub> \<subseteq>\<^isub>\<simeq> set arch"
 apply(subgoal_tac "\<exists>t. tameEnumFilter p = Some t \<and> Tries.set_of t \<subseteq>\<^isub>\<simeq> set arch")
- apply(metis TameEnum_tameEnumFilter eqi_gr.seteq_eqi_def eqi_gr.subseteq_eqi_trans)
+ apply(metis TameEnum_tameEnumFilter qle_gr.seteq_qle_def qle_gr.subseteq_qle_trans)
 apply(fastsimp intro!: samet_imp_iso_subseteq
   dest: inv_tries_tameEnumFilter tameEnumFilter_subseteq_TameEnum mgp_TameEnum mgp_pre_iso_test)
 done
