thys/Flyspeck-Tame/Quasi_Order.thy
@@ -1,0 +1,45 @@
+theory Quasi_Order
+imports Main
+begin
+
+locale quasi_order =
+fixes qle :: "'a \<Rightarrow> 'a \<Rightarrow> bool" (infix "\<preceq>" 60)
+assumes qle_refl[iff]: "x \<preceq> x"
+and qle_trans: "x \<preceq> y \<Longrightarrow> y \<preceq> z \<Longrightarrow> x \<preceq> z"
+begin
+
+definition in_qle :: "'a \<Rightarrow> 'a set \<Rightarrow> bool"  (infix "\<in>\<^isub>\<preceq>" 60) where
+ "x \<in>\<^isub>\<preceq> M \<equiv> \<exists>y \<in> M. x \<preceq> y"
+
+definition subseteq_qle :: "'a set \<Rightarrow> 'a set \<Rightarrow> bool" (infix "\<subseteq>\<^isub>\<preceq>" 60) where
+ "M \<subseteq>\<^isub>\<preceq> N \<equiv> \<forall>x \<in> M. x \<in>\<^isub>\<preceq> N"
+
+definition seteq_qle :: "'a set \<Rightarrow> 'a set \<Rightarrow> bool" (infix "=\<^isub>\<preceq>" 60) where
+ "M =\<^isub>\<preceq> N  \<equiv>  M \<subseteq>\<^isub>\<preceq> N \<and> N \<subseteq>\<^isub>\<preceq> M"
+
+lemmas "defs" = in_qle_def subseteq_qle_def seteq_qle_def
+
+lemma subseteq_qle_refl[simp]: "M \<subseteq>\<^isub>\<preceq> M"
+by(auto simp add: subseteq_qle_def in_qle_def)
+
+lemma subseteq_qle_trans: "A \<subseteq>\<^isub>\<preceq> B \<Longrightarrow> B \<subseteq>\<^isub>\<preceq> C \<Longrightarrow> A \<subseteq>\<^isub>\<preceq> C"
+by (simp add: subseteq_qle_def in_qle_def) (metis qle_trans)
+
+lemma empty_subseteq_qle[simp]: "{} \<subseteq>\<^isub>\<preceq> A"
+by (simp add: subseteq_qle_def)
+
+lemma subseteq_qleI2: "(!!x. x \<in> M \<Longrightarrow> EX y : N. x \<preceq> y) \<Longrightarrow> M \<subseteq>\<^isub>\<preceq> N"
+by (auto simp add: subseteq_qle_def in_qle_def)
+
+lemma subseteq_qleD2: "M \<subseteq>\<^isub>\<preceq> N \<Longrightarrow> x \<in> M \<Longrightarrow> EX y : N. x \<preceq> y"
+by (auto simp add: subseteq_qle_def in_qle_def)
+
+lemma seteq_qle_refl[iff]: "A =\<^isub>\<preceq> A"
+by (simp add: seteq_qle_def)
+
+lemma seteq_qle_trans: "A =\<^isub>\<preceq> B \<Longrightarrow> B =\<^isub>\<preceq> C \<Longrightarrow> A =\<^isub>\<preceq> C"
+by (simp add: seteq_qle_def) (metis subseteq_qle_trans)
+
+end
+
+end
